End-of-summer commit

timing/riscvTiming.v
@@ -81,6 +81,12 @@ Fixpoint decompose (instr low : N) (boundaries : list N) : n_tuple (length bound
 Compute mask_bit_section 63 3 4.
 Compute decompose 63 0 [2; 6]. *)
 
+Fixpoint contains (l:list N) (a:N) : bool :=
+    match l with
+      | nil => false
+      | b :: m => orb (b =? a) (contains m a)
+    end.
+
 (* https://www.cs.sfu.ca/~ashriram/Courses/CS295/assets/notebooks/RISCV/RISCV_CARD.pdf *)
 (* 
      31 30 29 28 27 26 25 24 23 22 21 20 19 18 17 16 15 14 13 12 11 10 09 08 07 06 05 04 03 02 01 00
@@ -173,6 +179,23 @@ Definition imm_Jtype (imm : N) :=
     ) in
     (imm_20 #<< 19) #| (imm_19_12 #<< 11) #| (imm_11 #<< 10) #| (imm_10_1 #<< 1).
 
+Definition decompose_CRtype (instr : N) : N * N * N * N :=
+    (
+        mask_bit_section instr 12 15 (* funct4 *),
+        mask_bit_section instr 7 11 (* rd/rs1 *),
+        mask_bit_section instr 2 6 (* rs2 *),
+        mask_bit_section instr 0 1 (* op *)
+    ).
+
+Definition decompose_CItype (instr : N) : N * N * N * N * N :=
+    (
+        mask_bit_section instr 13 15 (* funct3 *),
+        mask_bit_section instr 12 13 (* imm *),
+        mask_bit_section instr 7 11 (* rd/rs1 *),
+        mask_bit_section instr 2 6 (* imm *),
+        mask_bit_section instr 0 1 (* opp *)
+    ).
+
 (* https://en.wikichip.org/wiki/risc-v/registers *)
 (* Nvmd just use rv_varid *)
 Definition riscvvar_of_Z (reg : N) : option var :=
@@ -212,7 +235,8 @@ Definition riscvvar_of_Z (reg : N) : option var :=
     end.
 
 Definition riscv_opcode (instr : N) : N :=
-    mask_bit_section instr 0 6.
+    (* mask_bit_section instr 0 6. *)
+    instr #& 127.
 
 (* Necessary for max bound computations with register inputs *)
 Definition max32 : N := N.pow 2 32 - 1.
@@ -222,10 +246,10 @@ Definition max32 : N := N.pow 2 32 - 1.
 (*
     Inputs:
     - ML : Memory Latency of CPU
-    - prog : list of instructions comprising program
     - s : store representing CPU state
-    - addr : index into prog to decode
+    - instr : instruction to decode and compute cycles for
 *)
+
 Definition neorv32_cycles_upper_bound (ML : N) (s : store) (instr : N) : option N :=
     let reg_or_max (reg : N) : N := 
         match s (rv_varid reg) with
@@ -235,33 +259,30 @@ Definition neorv32_cycles_upper_bound (ML : N) (s : store) (instr : N) : option 
     in
     (* This is if/else instead of match, because matching on an N will expand its binary repr,
        which clogs up the goal space a bunch *)
+    (* Same with `contains` usage *)
     (* addi slti sltiu xori ori andi add sub slt sltu xor or and lui auipc : 2 *)
     let op := riscv_opcode instr in
     if op =? 51 then (* 0110011 : R-type *)
         let '(funct7, rs2, rs1, funct3, rd, opcode) := decompose_Rtype instr in
-        match funct3 with
-        | 0 | 2 | 3 | 4 | 6 | 7 =>
+        if contains [0;2;3;4;6;7] funct3 then
             (* add sub xor or and slt sltu *)
             Some 2%N
-        | _ => 
+        else
             (* sll srl sra : [ 3 + shamt/4 + shamt%4 ]*)
             (* shamt := rs2 *)
             (* Constant shift times are possible with FAST_SHIFT_EN or TINY_SHIFT_EN enabled *)
             Some (3 + (reg_or_max rs2 / 4) + ((reg_or_max rs2) mod 4))%N
-        end
     else if op =? 19 then (* 0010011 : I-type *)
         let '(imm, rs1, funct3, rd, opcode) := decompose_Itype instr in
-        match funct3 with
-        | 0 | 2 | 3 | 4 | 6 | 7 =>
+        if contains [0;2;3;4;6;7] funct3 then
             (* addi xori ori andi slti sltiu *)
             Some 2%N
-        | _ => 
+        else
             (* slli srli srai : [ 3 + shamt/4 + shamt%4 ] *)
             (* shamt := imm[0:4] *)
             (* Constant shift times are possible with FAST_SHIFT_EN or TINY_SHIFT_EN enabled *)
             let shamt := shamt_Itype imm in
             Some (3 + (shamt / 4) + (shamt mod 4))%N
-        end
     else if op =? 3 then (* 0000011 : I-type *)
         let '(imm, rs1, funct3, rd, opcode) := decompose_Itype instr in
         (* lb lh lw lbu lhu : [ 5 + (ML - 2) ] *)
@@ -274,7 +295,9 @@ Definition neorv32_cycles_upper_bound (ML : N) (s : store) (instr : N) : option 
         let '(imm_12_10_5, rs2, rs1, funct3, imm_4_1_11, opcode) := decompose_Btype instr in
         (* beq bne blt bge bltu bgeu : if taken then [ 5 + (ML - 1) ] else [ 3 ] *)
         if funct3 =? 0x0 then (* beq *)
-            match s (rv_varid rs1), s (rv_varid rs2) with
+            let rs1var := if rs1 =? 0 then VaN rs1 32 else s (rv_varid rs1) in
+            let rs2var := if rs2 =? 0 then VaN rs2 32 else s (rv_varid rs2) in
+            match rs1var, rs2var with
             | VaN r1 _, VaN r2 _ => Some
                 (if r1 =? r2 then
                     5 + (ML - 1)
@@ -283,7 +306,9 @@ Definition neorv32_cycles_upper_bound (ML : N) (s : store) (instr : N) : option 
             | _, _ => None
             end
         else if funct3 =? 0x1 then (* bne *)
-            match s (rv_varid rs1), s (rv_varid rs2) with
+            let rs1var := if rs1 =? 0 then VaN rs1 32 else s (rv_varid rs1) in
+            let rs2var := if rs2 =? 0 then VaN rs2 32 else s (rv_varid rs2) in
+            match rs1var, rs2var with
             | VaN r1 _, VaN r2 _ => Some
                 (if negb (r1 =? r2) then
                     5 + (ML - 1)
@@ -292,7 +317,9 @@ Definition neorv32_cycles_upper_bound (ML : N) (s : store) (instr : N) : option 
             | _, _ => None
             end
         else if funct3 =? 0x4 then (* blt *)
-            match s (rv_varid rs1), s (rv_varid rs2) with
+            let rs1var := if rs1 =? 0 then VaN rs1 32 else s (rv_varid rs1) in
+            let rs2var := if rs2 =? 0 then VaN rs2 32 else s (rv_varid rs2) in
+            match rs1var, rs2var with
             | VaN r1 _, VaN r2 _ => Some
                 (if Z.ltb (toZ 32 r1) (toZ 32 r2) then
                     5 + (ML - 1)
@@ -301,7 +328,9 @@ Definition neorv32_cycles_upper_bound (ML : N) (s : store) (instr : N) : option 
             | _, _ => None
             end
         else if funct3 =? 0x5 then (* bge *)
-            match s (rv_varid rs1), s (rv_varid rs2) with
+            let rs1var := if rs1 =? 0 then VaN rs1 32 else s (rv_varid rs1) in
+            let rs2var := if rs2 =? 0 then VaN rs2 32 else s (rv_varid rs2) in
+            match rs1var, rs2var with
             | VaN r1 _, VaN r2 _ => Some
                 (if Z.geb (toZ 32 r1) (toZ 32 r2) then
                     5 + (ML - 1)
@@ -310,7 +339,9 @@ Definition neorv32_cycles_upper_bound (ML : N) (s : store) (instr : N) : option 
             | _, _ => None
             end
         else if funct3 =? 0x6 then (* bltu *)
-            match s (rv_varid rs1), s (rv_varid rs2) with
+            let rs1var := if rs1 =? 0 then VaN rs1 32 else s (rv_varid rs1) in
+            let rs2var := if rs2 =? 0 then VaN rs2 32 else s (rv_varid rs2) in
+            match rs1var, rs2var with
             | VaN r1 _, VaN r2 _ => Some
                 (if r1 <? r2 then
                     5 + (ML - 1)
@@ -319,7 +350,9 @@ Definition neorv32_cycles_upper_bound (ML : N) (s : store) (instr : N) : option 
             | _, _ => None
             end
         else if funct3 =? 0x7 then (* bgeu *)
-            match s (rv_varid rs1), s (rv_varid rs2) with
+            let rs1var := if rs1 =? 0 then VaN rs1 32 else s (rv_varid rs1) in
+            let rs2var := if rs2 =? 0 then VaN rs2 32 else s (rv_varid rs2) in
+            match rs1var, rs2var with
             | VaN r1 _, VaN r2 _ => Some
                 (if negb (r1 <? r2)%N then
                     5 + (ML - 1)
@@ -339,12 +372,73 @@ Definition neorv32_cycles_upper_bound (ML : N) (s : store) (instr : N) : option 
     else if orb (op =? 55) (op =? 23) then (* 0110111 : U-type *) (* 0010111 : U-type *) Some 2%N
     else if op =? 115 then (* 1110011 : I-type *) Some 3%N
     (* TODO : Handle RISC-V Extensions *)
+    else if op =? 51 then (* 0110011 : R-type - RV32M Extension*)
+        Some 36%N
     else None.
 
-Definition add_loop_riscv_offset := 0xc.
-Definition add_loop_riscv : list N := [
-    0x00028863          	(* beqz	t0,1c <end> *);
-    0x00130313          	(* addi	t1,t1,1 *);
-    0x407282b3          	(* sub	t0,t0,t2 *);
-    0xfe000ae3          	(* beqz	zero,c <add> *)
-].
+(* Machinery to automate lifting - TODO replace with existing stuff *)
+Definition range (start stop : N) : list N :=
+    let fix aux (n : nat) :=
+        match n with
+        | O => []
+        | S n' => n :: aux n'
+        end
+    in List.rev (List.map (fun n => start + 4 * N.of_nat (n - 1)) (aux (N.to_nat (1 + (stop - start) / 4)))).
+
+Definition rv_stmt' m a :=
+    (* removed getmem here. why was it giving nops? *)
+    rv2il a match a mod 4 with 0 => rv_decode (m a) | _ => R5_InvalidI end.
+
+Definition il_list (prog : store -> addr -> N) (prog_start prog_end : N) :=
+    List.map (fun a => (a, Some (4, rv_stmt' (prog (fun _ => VaN 0 32)) a))) (range prog_start prog_end).
+
+Definition update_prog old_prog (a : addr) newval : program :=
+    fun s a' => if N.eqb a a' then newval else old_prog s a'.
+
+Fixpoint program_of_list l :=
+        match l with 
+        | nil => fun _ _ => None    
+        | h :: t => update_prog (program_of_list t) (fst h) (snd h)
+        end.
+
+Definition lift_via_list (f : store -> addr -> N) (prog_start prog_end : N) : program :=
+    program_of_list (il_list f prog_start prog_end).
+
+Definition lift_riscv (f : store -> addr -> N) s a :=
+    Some (4, rv2il a (rv_decode (f s a))).
+
+(* Timing machinery *)
+Definition cycle_count_of_trace (time_of_addr : store -> addr -> N) (t : trace) : N :=
+    List.fold_left N.add (List.map 
+        (fun '(e, s) => match e with 
+            | Addr a => time_of_addr s a
+            | Raise n => max32
+            end) t) 0.
+
+Lemma fold_left_cons : forall {X : Type} (t : list X) (h : X) (f : X -> X -> X) (base : X) 
+    (Comm : forall a b, f a b = f b a) (Assoc : forall a b c, f a (f b c) = f (f a b) c),
+    List.fold_left f (h :: t) base = f h (List.fold_left f t base).
+Proof.
+    induction t; intros.
+    - simpl. now rewrite Comm.
+    - simpl in *. rewrite IHt, IHt, IHt,
+        Assoc, Assoc, (Comm a h); auto.
+Qed.
+
+Lemma cycle_count_of_trace_single :
+    forall (e : exit) (s : store) time_of_addr,
+    cycle_count_of_trace time_of_addr [(e, s)] = 
+        match e with 
+        | Addr a => time_of_addr s a
+        | Raise n => max32
+        end.
+Proof. reflexivity. Qed.
+
+Lemma cycle_count_of_trace_cons :
+    forall (t : trace) (e : exit) (s : store) time_of_addr,
+    cycle_count_of_trace time_of_addr ((e, s) :: t) = cycle_count_of_trace time_of_addr [(e, s)] + cycle_count_of_trace time_of_addr t.
+Proof.
+    intros. unfold cycle_count_of_trace at 2. rewrite map_cons, fold_left_cons; try lia. simpl.
+    unfold cycle_count_of_trace at 1. rewrite map_cons, fold_left_cons. rewrite N.add_0_r. reflexivity.
+    lia. lia.
+Qed.
