timing/examples/FreeRTOS_tasks_proofs.v
@@ -1,0 +1,315 @@
+Require Import lifted_RTOSDemo.
+Require Import riscvTiming.
+Import RISCVNotations.
+
+Variable ML : N.
+Variable ML_pos : 1 <= ML.
+
+Module riscv_toa.
+    Definition time_of_addr (s : store) (a : addr) : N :=
+        match neorv32_cycles_upper_bound ML s (vTaskSwitchContext s a) with
+        | Some x => x | _ => 0 end.
+End riscv_toa.
+
+Module riscvT := MakeTimingContents riscvTiming riscv_toa.
+Export riscvT.
+
+Definition cycle_count_of_trace := cycle_count_of_trace time_of_addr.
+
+Definition time_mem : N :=
+    5 + (ML - 2).
+
+Definition time_branch : N :=
+    5 + (ML - 1).
+
+Definition uxSchedulerSuspended (gp : N) (mem : addr -> N) : N :=
+    mem â¹[2144 + gp].
+    (* This should actually be the below expression. Unclear on whether lifter
+       has bug, seems like it isn't treating immediate as signed
+    *)
+    (* mem â¹[gp - 1952]. *)
+
+Definition addr_xYieldPendings (gp : N) : N :=
+    gp - 1932.
+
+Definition pxCurrentTCB (gp : N) (mem : addr -> N) : N :=
+    mem â¹[2200 + gp].
+    (* Same as above *)
+    (* mem â¹[gp - 1896]. *)
+
+Definition uxTopReadyPriority (gp : N) (mem : addr -> N) : N :=
+    mem â¹[gp - 1920].
+
+Definition addr_pxReadyTasksLists (gp : N) : N :=
+    gp - 924.
+
+(* 
+(* <vTaskSwitchContext> *)
+    | 0x800015e0 => 0x8601a703 (* lw a4,-1952(gp) # 80080060 <uxSchedulerSuspended>  *) time_mem
+    | 0x800015e4 => 0x00070863 (* beqz a4,800015f4 <vTaskSwitchContext+0x14>  *)
+        if uxSchedulerSuspended (s R_GP) mem =? 0 then time_branch else 3
+    | 0x800015e8 => 0x00100713 (* li a4,1  *)                                           2
+    | 0x800015ec => 0x86e1aa23 (* sw a4,-1932(gp) # 80080074 <xYieldPendings>  *)       time_mem
+    | 0x800015f0 => 0x00008067 (* ret  *)                                               time_branch
+    | 0x800015f4 => 0xff010113 (* add sp,sp,-16  *)                                     2
+    | 0x800015f8 => 0x8601aa23 (* sw zero,-1932(gp) # 80080074 <xYieldPendings>  *)     time_mem
+    | 0x800015fc => 0x01212023 (* sw s2,0(sp)  *)                                       time_mem
+    | 0x80001600 => 0x8981a783 (* lw a5,-1896(gp) # 80080098 <pxCurrentTCB>  *)         time_mem
+    | 0x80001604 => 0xa5a5a737 (* lui a4,0xa5a5a  *)                                    2
+    | 0x80001608 => 0x00112623 (* sw ra,12(sp)  *)                                      time_mem
+    | 0x8000160c => 0x0307a783 (* lw a5,48(a5)  *)                                      time_mem
+    | 0x80001610 => 0x00812423 (* sw s0,8(sp)  *)                                       time_mem
+    | 0x80001614 => 0x00912223 (* sw s1,4(sp)  *)                                       time_mem
+    | 0x80001618 => 0x0007a603 (* lw a2,0(a5)  *)                                       time_mem
+    | 0x8000161c => 0x5a570713 (* add a4,a4,1445 # a5a5a5a5 <_stack_top+0x259c48b7>  *) 2
+    | 0x80001620 => 0x00e61e63 (* bne a2,a4,8000163c <vTaskSwitchContext+0x5c>  *)
+        if mem â¹[mem â¹[48 + pxCurrentTCB gp mem]] !=? 0xa5a5a5a5 then time_branch else 3
+    | 0x80001624 => 0x0047a683 (* lw a3,4(a5)  *)                                       time_mem
+    | 0x80001628 => 0x00c69a63 (* bne a3,a2,8000163c <vTaskSwitchContext+0x5c>  *)
+        if mem â¹[4 + (48 + pxCurrentTCB gp mem)] !=? mem â¹[mem â¹[48 + pxCurrentTCB gp mem]] then time_branch else 3
+    | 0x8000162c => 0x0087a703 (* lw a4,8(a5)  *)                                       time_mem
+    | 0x80001630 => 0x00d71663 (* bne a4,a3,8000163c <vTaskSwitchContext+0x5c>  *)
+        if mem â¹[8 + (48 + pxCurrentTCB gp mem)] !=? mem â¹[4 + (48 + pxCurrentTCB gp mem)] then time_branch else 3
+    | 0x80001634 => 0x00c7a783 (* lw a5,12(a5)  *)                                      time_mem
+    | 0x80001638 => 0x00e78a63 (* beq a5,a4,8000164c <vTaskSwitchContext+0x6c>  *)
+        if mem â¹[12 + (48 + pxCurrentTCB gp mem)] !=? mem â¹[8 + (48 + pxCurrentTCB gp mem)] then time_branch else 3
+    | 0x8000163c => 0x8981a583 (* lw a1,-1896(gp) # 80080098 <pxCurrentTCB>  *)         time_mem
+    | 0x80001640 => 0x8981a503 (* lw a0,-1896(gp) # 80080098 <pxCurrentTCB>  *)         time_mem
+    | 0x80001644 => 0x03458593 (* add a1,a1,52  *)                                      2
+    | 0x80001648 => 0x429100ef (* jal 80012270 <vApplicationStackOverflowHook>  *)      time_branch + timeof(vApplicationStackOverflowHook)
+    | 0x8000164c => 0x8801a503 (* lw a0,-1920(gp) # 80080080 <uxTopReadyPriority>  *)   time_mem
+    | 0x80001650 => 0x01f00493 (* li s1,31  *)                                          2
+    | 0x80001654 => 0x02c120ef (* jal 80013680 <__clzsi2>  *)                           time_branch + timeof(__clzsi2)
+    | 0x80001658 => 0x40a484b3 (* sub s1,s1,a0  *)                                      2
+    | 0x8000165c => 0x01400713 (* li a4,20  *)                                          2
+    | 0x80001660 => 0x02e48733 (* mul a4,s1,a4  *)                                      2
+    | 0x80001664 => 0xc6418793 (* add a5,gp,-924 # 80080464 <pxReadyTasksLists>  *)     2
+    | 0x80001668 => 0xc6418413 (* add s0,gp,-924 # 80080464 <pxReadyTasksLists>  *)     2
+    | 0x8000166c => 0x00e787b3 (* add a5,a5,a4  *)                                      2
+    | 0x80001670 => 0x0007a783 (* lw a5,0(a5)  *)                                       time_mem
+    | 0x80001674 => 0x00079c63 (* bnez a5,8000168c <vTaskSwitchContext+0xac>  *)
+        if mem â¹[(GP - 924) + ((31 - mem â¹[GP - 1920]) * 20)] !=? 0 then time_branch else 3
+    | 0x80001678 => 0x000015b7 (* lui a1,0x1  *)                                        2
+    | 0x8000167c => 0x80014537 (* lui a0,0x80014  *)                                    2
+    | 0x80001680 => 0x41358593 (* add a1,a1,1043 # 1413 <__stack_size+0x12b5>  *)       2
+    | 0x80001684 => 0xbd050513 (* add a0,a0,-1072 # 80013bd0 <_etext>  *)               2
+    | 0x80001688 => 0x409100ef (* jal 80012290 <vAssertCalled>  *)                      time_branch + timeof(vAssertCalled)
+    | 0x8000168c => 0x01400793 (* li a5,20  *)                                          2
+    | 0x80001690 => 0x02f487b3 (* mul a5,s1,a5  *)                                      2
+    | 0x80001694 => 0x00f40733 (* add a4,s0,a5  *)                                      2
+    | 0x80001698 => 0x00472683 (* lw a3,4(a4)  *)                                       time_mem
+    | 0x8000169c => 0x00878793 (* add a5,a5,8  *)                                       2
+    | 0x800016a0 => 0x00f407b3 (* add a5,s0,a5  *)                                      2
+    | 0x800016a4 => 0x0046a683 (* lw a3,4(a3)  *)                                       time_mem
+    | 0x800016a8 => 0x00d72223 (* sw a3,4(a4)  *)                                       time_mem
+    | 0x800016ac => 0x00f69663 (* bne a3,a5,800016b8 <vTaskSwitchContext+0xd8>  *)
+        if mem â¹[4 + mem â¹[4 + (addr_pxReadyTasksLists + ((31 - uxTopReadyPriority) * 20))]] !=? 
+            (addr_pxReadyTasksLists + (((31 - uxTopReadyPriority) * 20) + 8)) then time_branch else 3
+    | 0x800016b0 => 0x00c72783 (* lw a5,12(a4)  *)                                      time_mem
+    | 0x800016b4 => 0x00f72223 (* sw a5,4(a4)  *)                                       time_mem
+    | 0x800016b8 => 0x01400793 (* li a5,20  *)                                          2
+    | 0x800016bc => 0x02f484b3 (* mul s1,s1,a5  *)                                      2
+    | 0x800016c0 => 0x00c12083 (* lw ra,12(sp)  *)                                      time_mem
+    | 0x800016c4 => 0x00940433 (* add s0,s0,s1  *)                                      2
+    | 0x800016c8 => 0x00442783 (* lw a5,4(s0)  *)                                       time_mem
+    | 0x800016cc => 0x00812403 (* lw s0,8(sp)  *)                                       time_mem
+    | 0x800016d0 => 0x00412483 (* lw s1,4(sp)  *)                                       time_mem
+    | 0x800016d4 => 0x00c7a783 (* lw a5,12(a5)  *)                                      time_mem
+    | 0x800016d8 => 0x88f1ac23 (* sw a5,-1896(gp) # 80080098 <pxCurrentTCB>  *)         time_mem
+    | 0x800016dc => 0x8981a783 (* lw a5,-1896(gp) # 80080098 <pxCurrentTCB>  *)         time_mem
+    | 0x800016e0 => 0x00012903 (* lw s2,0(sp)  *)                                       time_mem
+    | 0x800016e4 => 0x01010113 (* add sp,sp,16  *)                                      2
+    | 0x800016e8 => 0x00008067 (* ret  *)                                               5 + (ML - 1)
+*)
+
+Definition vTaskSwitchContext_exit (t:trace) :=
+  match t with (Addr a,_)::_ => match a with
+  | 0x800015f0 | 0x800016e8 => true
+  | _ => false
+  end | _ => false end.
+
+Definition timing_postcondition (t : trace) (gp : N) (mem : addr -> N) : Prop :=
+    cycle_count_of_trace t = if (uxSchedulerSuspended gp mem) =? 0 then 77 else 5 + time_branch + 2 * time_mem.
+
+Notation "x !=? y" := (negb (x =? y)) (at level 70, no associativity) : N_scope.
+
+Definition gp_sp_noverlap (gp sp : N) : Prop :=
+    ~overlap 32 gp __global_size sp vTaskSwitchContext_stack_frame_size.
+
+Definition vTaskSwitchContext_timing_invs (_ : store) (p : addr) (base_sp : N) (t:trace) :=
+match t with (Addr a, s) :: t' => match a with
+    | 0x800015e4 => Some (
+        exists mem gp, s V_MEM32 = âmem /\ s R_GP = â¹gp /\ s R_SP = â¹base_sp /\ s R_A4 = â¹(uxSchedulerSuspended gp mem) /\ gp_sp_noverlap gp base_sp /\
+        cycle_count_of_trace t' = time_mem)
+    (* The proof expressions get big, so throw in a few intermediate invariants to constrain the goal space's size *)
+    (* | 0x80001610 => Some (exists mem gp, s V_MEM32 = âmem /\ s R_GP = â¹gp /\ s R_SP = â¹(base_sp â 16)  /\ gp_sp_noverlap gp base_sp /\
+        s R_A5 = â¹(mem â¹[48 + pxCurrentTCB gp mem]) /\
+        s R_A4 = â¹(0xa5a5a) /\
+        cycle_count_of_trace t' = 4 + 6 * time_mem + time_branch
+    ) *)
+    | 0x80001620 => Some (exists mem gp, s V_MEM32 = âmem /\ s R_GP = â¹gp /\ s R_SP = â¹(base_sp â 16) /\
+        s R_A5 = â¹(mem â¹[48 + pxCurrentTCB gp mem]) /\
+        s R_A2 = â¹(mem â¹[mem â¹[48 + pxCurrentTCB gp mem]]) /\
+        s R_A4 = â¹((0xa5a5a << 12) + 1445) /\
+        cycle_count_of_trace t' = 6 + 9 * time_mem + time_branch)
+    | 0x8000163c => Some (exists mem gp, s V_MEM32 = âmem /\ s R_GP = â¹gp /\
+        s R_A5 = â¹(mem â¹[48 + pxCurrentTCB gp mem]) /\
+        cycle_count_of_trace t' = 6 + 9 * time_mem + time_branch + 
+            if mem â¹[mem â¹[ 48 + pxCurrentTCB gp mem ]] !=? 0xa5a5a5a5 then time_branch else 3
+    )
+    | 0x80001648 => Some (exists mem gp, s V_MEM32 = âmem /\ s R_GP = â¹gp /\ cycle_count_of_trace t' = 8 + 11 * time_mem + 2 * time_branch)
+    | 0x80001628 => Some (exists mem gp, s V_MEM32 = âmem /\ s R_GP = â¹gp /\ 
+        cycle_count_of_trace t' = 
+            if (mem â¹[ mem â¹[ 48 + pxCurrentTCB gp mem ] ] !=? 0xa5a5a5a5) then 
+                (9 + 10 * time_mem + time_branch)
+            else
+                ((if mem â¹[ mem â¹[ 48 + pxCurrentTCB gp mem ] ] !=? 0xa5a5a5a5 then time_branch else 3) + 
+                    (6 + 10 * time_mem + time_branch)))
+    | 0x80001630 | 0x80001638 
+        | 0x80001654 | 0x80001674 | 0x80001688 | 0x800016ac => Some (cycle_count_of_trace t' = 99)
+    | 0x800015f0 | 0x800016e8 => Some (
+        exists mem gp, s V_MEM32 = âmem /\ s R_GP = â¹gp /\
+            timing_postcondition t gp mem)
+    | _ => None end
+| _ => None
+end.
+
+Definition lifted_vTaskSwitchContext : program :=
+    (* lift_via_list vTaskSwitchContext start_vTaskSwitchContext end_vTaskSwitchContext. *)
+    lift_riscv vTaskSwitchContext.
+
+Compute lifted_vTaskSwitchContext empty_store start_vTaskSwitchContext.
+
+Theorem vTaskSwitchContext_welltyped: welltyped_prog rvtypctx lifted_vTaskSwitchContext.
+(* Proof. Picinae_typecheck. Qed. *)
+Admitted.
+
+Ltac unfold_decompose :=
+    cbv [decompose_Btype decompose_Itype decompose_Jtype decompose_Rtype 
+        decompose_Stype decompose_Utype mask_bit_section]; simpl (_ .& _).
+Tactic Notation "unfold_decompose" "in" hyp(H) :=
+    cbv [decompose_Btype decompose_Itype decompose_Jtype decompose_Rtype 
+        decompose_Stype decompose_Utype mask_bit_section] in H; simpl (_ .& _) in H.
+
+Ltac unfold_time_of_addr :=
+    cbv [time_of_addr neorv32_cycles_upper_bound]; cbn - [getmem].
+Tactic Notation "unfold_time_of_addr" "in" hyp(H) :=
+    cbv [time_of_addr neorv32_cycles_upper_bound] in H; cbn - [getmem] in H.
+
+Ltac unfold_cycle_count_list :=
+    unfold cycle_count_of_trace; repeat rewrite cycle_count_of_trace_cons, cycle_count_of_trace_single; fold cycle_count_of_trace.
+
+Ltac fold_times :=
+    fold time_mem; fold time_branch.
+
+Ltac hammer :=
+    unfold_cycle_count_list; unfold_time_of_addr; unfold_decompose; fold_times; psimpl; try lia.
+
+Arguments N.add _ _ : simpl nomatch.
+Arguments N.mul _ _ : simpl nomatch.
+
+Theorem vTaskSwitchContext_timing:
+  forall s p t s' x' gp sp
+         (ENTRY: startof t (x',s') = (Addr start_vTaskSwitchContext,s)) (* Define the entry point of the function *)
+         (MDL: models rvtypctx s)
+         (GP : s R_GP = â¹gp)
+         (SP : s R_SP = â¹sp)
+         (GP_SP_FAR : gp_sp_noverlap gp sp),
+  satisfies_all 
+    lifted_vTaskSwitchContext                                 (* Provide lifted code *)
+    (vTaskSwitchContext_timing_invs s p sp)                  (* Provide invariant set *)
+    vTaskSwitchContext_exit                                   (* Provide exit point *)
+  ((x',s')::t).
+Proof using.
+    intros.
+    apply prove_invs.
+    Local Ltac step := time rv_step.
+    Local Ltac handle_ex := eexists; eexists; repeat split; try eassumption.
+    Local Ltac destruct_pre PRE := destruct PRE as [mem [gp [MEM [GP [GP_SP_FAR Cycles]]]]].
+
+    (* Base case *)
+    simpl. rewrite ENTRY. step. rename m into mem.
+    exists mem, gp. repeat split; assumption.
+
+    (* Inductive step setup *)
+    intros.
+    eapply startof_prefix in ENTRY; try eassumption.
+    eapply preservation_exec_prog in MDL; try eassumption; [idtac|apply vTaskSwitchContext_welltyped].
+    clear - PRE MDL. rename t1 into t. rename s1 into s'.
+
+    (* Meat of proof starts here *)
+    destruct_inv 32 PRE.
+
+    (* 0x800015e4 *)
+    destruct PRE as [mem [gp [MEM [GP [SP [A4 [GP_SP_FAR Cycles]]]]]]].
+    step. step. step. step. step. step. step. step. step. step. step. step.
+    do 2 eexists. repeat split. unfold msub. now psimpl.
+        unfold pxCurrentTCB. admit. admit.
+    hammer. rewrite A4, BC, Cycles. lia.
+
+    (* 0x800015e8 *)
+    step. step. handle_ex.
+    unfold timing_postcondition. unfold uxSchedulerSuspended. psimpl. 
+    hammer. fold (uxSchedulerSuspended gp mem). rewrite A4, BC, Cycles. lia.
+    
+    (* 0x80001620 *)
+    destruct PRE as [mem [gp [MEM [GP [SP [A5 [A2 [A4 Cycles]]]]]]]].
+    step. handle_ex.
+        hammer. change ((678490 << 12) + 1445) with 0xa5a5a5a5 in *.
+        rewrite A2, A4, Cycles. lia.
+    step. handle_ex.
+        hammer. change ((678490 << 12) + 1445) with 0xa5a5a5a5 in *.
+        rewrite A2, A4, Cycles, BC. lia.
+
+    (* 0x80001620 *)
+    destruct PRE as [mem [gp [MEM [GP Cycles]]]].
+    step.
+        handle_ex. hammer. rewrite Hsv, A2, Cycles.
+
+    (* 0x80001624 *)
+    step. hammer. rewrite Hsv0, Hsv, BC, PRE. lia.
+
+    (* 0x80001628 *)
+    step. step. step. step. hammer. rewrite Hsv0, Hsv, BC, PRE. psimpl.
+
+    step. step. step. step. step. step. step. step. step. step. step. step.
+        hammer. rewrite Hsv, BC.
+        rewrite PRE. lia.
+    step. step. step. step. step. step. step. step.
+        hammer. rewrite Hsv, BC.
+        rewrite PRE. lia.
+
+    (* 0x2ddc *)
+    step.
+    step. step. step. step. step. step. step. step. step.
+        (* Infinite loop *) admit.
+    step. step. step. step. hammer. rewrite Hsv, Hsv0, BC, PRE. lia.
+
+    (* 0x2df0 *)
+    step. step. step. step. step. step. step. step. step. step.
+        (* Infinite loop *) admit.
+    step. step. step. step.
+        hammer. rewrite Hsv, Hsv0, BC, PRE. lia.
+
+    (* 0x2e04 *)
+    step. step. step. step. step. step. step. step. step. step.
+        (* Infinite loop *) admit.
+    step. step. step. step.
+        hammer. rewrite Hsv, Hsv0, BC, PRE. lia.
+
+    (* 0x2e18 *)
+    step. step. step. step. step.
+        (* Infinite loop *) admit.
+    step. step. step. step. step. step. step. step. step.
+        (* Infinite loop *) admit.
+
+    (* 0x2e90 *)
+    step. step. step. step. step. step. step. step. step. step. step. step. step. step.
+        step. step. step. step. step.
+        hammer. rewrite Hsv, BC, PRE. lia.
+    step. step. step. step. step.
+        (* Infinite loop *) admit.
+    
+    (* 0x2ef4 *)
+    step. step. step. step. step. step. step. step. step. step. step. step.
+        hammer. rewrite Hsv, Hsv0, BC, PRE. psimpl. 
