timing/examples/riscv_addloop_proof.v
@@ -1,0 +1,288 @@
+Require Import Picinae_riscv.
+Require Import riscvTiming.
+Import RISCVNotations.
+Require Import NArith.
+Require Import List.
+
+Import ListNotations.
+Open Scope N_scope.
+
+(* 
+    To create this function, I:
+    - Wrote some assembly
+
+            andi t0, t0, 5
+            andi t1, t1, 9
+        start:
+            andi t2, t2, 1
+            andi t3, t3, 0
+        add:
+            beq t0, t3, end
+            addi t1, t1, 1
+            sub t0, t0, t2
+            beq t3, t3, add
+        end:
+
+    - Assembled it using a RISC-V cross-assembler
+        https://github.com/riscv-collab/riscv-gnu-toolchain
+        You can probably do this with clang instead of building a GCC (takes a long time)
+      Command:
+        charles@derelict:~/riscv-gnu-toolchain$ /usr/bin/riscv64-unknown-linux-gnu/bin/as addloop.s -o addloop.o
+
+    - Dumped the assembled code
+      Command:
+        charles@derelict:~/riscv-gnu-toolchain$ /usr/bin/riscv64-unknown-linux-gnu/bin/objdump addloop.o -D
+      This prints out a bunch of text:
+
+        addloop.o:     file format elf64-littleriscv
+
+
+        Disassembly of section .text:
+
+        0000000000000000 <start-0x8>:
+        0:	00506293          	ori	t0,zero,5
+        4:	00906313          	ori	t1,zero,9
+
+        0000000000000008 <start>:
+        8:	00106393          	ori	t2,zero,1
+        c:	000e7e13          	andi	t3,t3,0
+
+        0000000000000010 <add>:
+        10:	01c28863          	beq	t0,t3,20 <end>
+        14:	00130313          	addi	t1,t1,1
+        18:	407282b3          	sub	t0,t0,t2
+        1c:	ffce0ae3          	beq	t3,t3,10 <add>
+
+    - Manually copied the addresses and hex-encoded instructions to the function below
+      I ignored the <start-0x8> section because it's just a test case and not a part of the program logic
+*)
+Definition add_loop_riscv (_ : store) (a : addr) : N :=
+    match a with
+    | 0x8  => 0x00106393 (* ori     t2,zero,1 *)
+    | 0xc  => 0x000e7e13 (* andi	t3,t3,0 *)
+    | 0x10 => 0x01c28863 (* beq	t0,t3,20 <end> *)
+    | 0x14 => 0x00130313 (* addi	t1,t1,1 *)
+    | 0x18 => 0x407282b3 (* sub	t0,t0,t2 *)
+    | 0x1c => 0xffce0ae3 (* beq	t3,t3,10 <add> *)
+    | _ => 0 
+    end.
+Definition add_loop_start : N := 0x8.
+Definition add_loop_end   : N := 0x1c.
+
+(*
+    Now to define correctness. Let's ignore most of the machinery and just look
+    at what the invariants say:
+
+    We have some input numbers x and y. These aren't machine numbers, but Coq
+    binary numbers. The insight here is that the semantics of the addloop code
+    should implement the functional behavior of some ideal addition function.
+    This gives us our postcondition, which calls coq's N.add function (wrapped
+    in a 'mod 2^32', hence the circle plus).
+*)
+Definition postcondition (s : store) (x y : N) :=
+    s R_T1 = â¹(x â y).
+
+(*
+    We really only have one invariant here (because we only have one loop in the
+    code), and that's at address 0x10. It says:
+        'given that registers T0 and T1 contain some numbers t0 and t1, and
+         that registers T2 and T3 contain 1 and 0 respectively, the modular
+         sum of t0 and t1 equals the modular sum of x and y'
+    Why did I choose this invariant? What is an invariant?
+
+    TLDR: an invariant is a statement that is true throughout each iteration of
+    a loop. Invariants carry important information throughout the proof that
+    would otherwise be lost as the interpreter leaves a loop. So if the loop
+    does anything that impacts the correctness of the function (hint: they
+    usually do), then that loop's invariant needs to encode that information.
+
+    I chose the invariant that t0 + t1 = x + y because it's a direct generalization
+    of the postcondition. We know that t0 is repeatedly subtracted from until it
+    hits 0, leaving the sum in t1. So t0 + t1 eventually becomes 0 + (x + y).
+
+    TODO : Hamlen should check explanation after this point
+    We place an invariant at the entrance to the function just for setup, and
+    we place our postcondition at the exit point of the function.
+*)
+Definition addloop_correctness_invs (_ : store) (p : addr) (x y : N) (t:trace) :=
+    match t with (Addr a, s) :: _ => match a with
+        | 0x8  => Some (s R_T0 = VaN x 32 /\ s R_T1 = VaN y 32)
+        | 0x10 => Some (exists t0 t1, 
+            s R_T0 = â¹t0 /\ s R_T1 = â¹t1 /\ s R_T2 = â¹1 /\ s R_T3 = â¹0 /\ 
+                t0 â t1 = x â y)
+        | 0x20 => Some (postcondition s x y)
+        | _ => None end
+    | _ => None
+    end.
+
+(* Let's also define the exit point of addloop *)
+Definition addloop_exit (t:trace) :=
+  match t with (Addr a,_)::_ => match a with
+  | 0x20 => true
+  | _ => false
+  end | _ => false end.
+
+(*
+    TODO : FIX JANK
+    This is all machinery I use to lift code. I converted the above function into a list,
+    transformed it into Picinae IL. There should be a much easier way to just map IL onto
+    the function above instead of all of this. Or maybe not. Hamlen question.
+*)
+Definition lifted_addloop := lift_via_list add_loop_riscv add_loop_start add_loop_end.
+
+(*
+    And now for the proofs:
+*)
+
+(* Well-typedness of the lifted code, automatic *)
+Theorem addloop_welltyped: welltyped_prog rvtypctx lifted_addloop.
+Proof. Picinae_typecheck. Qed.
+
+(* Our partial correctness proof (partial because it assumes termination) *)
+Theorem addloop_partial_correctness:
+  forall s p t s' x' a b
+         (ENTRY: startof t (x',s') = (Addr 0x8,s)) (* Define the entry point of the function *)
+         (MDL: models rvtypctx s)
+         (T0: s R_T0 = VaN a 32)                   (* Tie the contents of T0 to a *)
+         (T1: s R_T1 = VaN b 32),                  (* Tie the contents of T1 to b *)
+  satisfies_all 
+    lifted_addloop                                 (* Provide lifted code *)
+    (addloop_correctness_invs s p a b)             (* Provide invariant set *)
+    addloop_exit                                   (* Provide exit point *)
+  ((x',s')::t).
+Proof.
+    Local Ltac step := time rv_step.
+
+    intros.
+    apply prove_invs.
+
+    (* Base case *)
+    simpl. rewrite ENTRY. step. split.
+        assumption.
+        assumption.
+
+    (* Inductive step setup *)
+    intros.
+    eapply startof_prefix in ENTRY; try eassumption.
+    eapply preservation_exec_prog in MDL; try (eassumption || apply addloop_welltyped).
+    clear - PRE MDL. rename t1 into t. rename s1 into s'.
+
+    (* Meat of proof starts here *)
+    destruct_inv 32 PRE.
+
+    (* Starting from our entrypoint at address 6, we'll do some setup and then
+       step to the next invariant *)
+    destruct PRE as [T0 T1]. step. step.
+    (* This goal is the invariant at 0x10 and has taken us to the case in which
+       the loop has just started *)
+    (* A big mess, but most of this is solvable with reflexivity *)
+    exists a, b. repeat split.
+        assumption.
+        assumption.
+
+    (* We now have to deal with the cases where the loop terminates and where it
+       loops around. Notice we get our invariant as an assumption! *)
+    destruct PRE as [t0 [t1 [T0 [T1 [T2 [T3 Eq]]]]]].
+    (* Termination case - time to prove the postcondition *)
+    step.
+        rewrite N.eqb_eq in BC. subst. psimpl in Eq.
+        unfold postcondition. psimpl. rewrite <- Eq. assumption.
+    (* Loop case - prove the invariant again *)
+    step. step. step.
+        rewrite N.eqb_neq in BC. exists (t0 â 1), (1 â t1). repeat split.
+        psimpl. assumption.
+Qed.
+
+(* Timing proof - lots of machinery here has yet to be modularized *)
+Variable ML : N.
+Variable ML_pos : 1 <= ML.
+
+Module riscv_toa.
+    Definition time_of_addr (s : store) (a : addr) : N :=
+        match neorv32_cycles_upper_bound ML s (add_loop_riscv s a) with
+        | Some x => x | _ => 0 end.
+End riscv_toa.
+
+Module riscvT := MakeTimingContents riscvTiming riscv_toa.
+Export riscvT.
+
+Definition cycle_count_of_trace := cycle_count_of_trace time_of_addr.
+
+Arguments N.add _ _ : simpl nomatch.
+
+Definition addloop_timing_invs (_ : store) (p : addr) (x y : N) (t:trace) :=
+match t with (Addr a, s) :: t' => match a with
+    | 0xc  => Some (s R_T0 = â¹x /\ s R_T2 = â¹1 /\ cycle_count_of_trace t = 2 + 2)
+    | 0x10 => Some (exists t0, s R_T0 = â¹t0 /\ s R_T2 = â¹1 /\ s R_T3 = â¹0 /\ t0 <= x /\
+        cycle_count_of_trace t' = 4 + (x - t0) * (12 + (ML - 1)))
+        (* 2 + 2 + (x - t0) * (3 + 2 + 2 + (5 + (ML - 1)) *)
+    | 0x20 => Some (cycle_count_of_trace t' = 9 + (ML - 1) + x * (12 + (ML - 1)))
+        (* 2 + 2 + (5 + (ML - 1)) + x * (3 + 2 + 2 + (5 + (ML - 1))) *)
+    | _ => None end
+| _ => None
+end.
+
+Ltac unfold_decompose :=
+    cbv [decompose_Btype decompose_Itype decompose_Jtype decompose_Rtype decompose_Stype decompose_Utype mask_bit_section];
+        simpl (_ .& _).
+Tactic Notation "unfold_decompose" "in" hyp(H) :=
+    cbv [decompose_Btype decompose_Itype decompose_Jtype decompose_Rtype decompose_Stype decompose_Utype mask_bit_section] in H;
+        simpl (_ .& _) in H.
+
+Ltac unfold_time_of_addr :=
+    cbv [time_of_addr neorv32_cycles_upper_bound]; simpl.
+Tactic Notation "unfold_time_of_addr" "in" hyp(H) :=
+    cbv [time_of_addr neorv32_cycles_upper_bound] in H; simpl in H.
+
+Ltac unfold_cycle_count_list :=
+    unfold cycle_count_of_trace; repeat rewrite cycle_count_of_trace_cons, cycle_count_of_trace_single; fold cycle_count_of_trace.
+
+Theorem addloop_timing:
+  forall s p t s' x' a b
+         (ENTRY: startof t (x',s') = (Addr 0x8,s)) (* Define the entry point of the function *)
+         (MDL: models rvtypctx s)
+         (T0: s R_T0 = VaN a 32)                   (* Tie the contents of T0 to a *)
+         (T1: s R_T1 = VaN b 32),                  (* Tie the contents of T1 to b *)
+  satisfies_all 
+    lifted_addloop                                 (* Provide lifted code *)
+    (addloop_timing_invs s p a b)                  (* Provide invariant set *)
+    addloop_exit                                   (* Provide exit point *)
+  ((x',s')::t).
+Proof using.
+    intros.
+    apply prove_invs.
+
+    (* Base case *)
+    simpl. rewrite ENTRY. step. now repeat split.
+
+    (* Inductive step setup *)
+    intros.
+    eapply startof_prefix in ENTRY; try eassumption.
+    eapply preservation_exec_prog in MDL; try (eassumption || apply addloop_welltyped).
+    clear - PRE MDL. rename t1 into t. rename s1 into s'.
+
+    (* Meat of proof starts here *)
+    destruct_inv 32 PRE.
+
+    (* Addr 0xc *)
+    destruct PRE as [T0 [T2 Cycles]].
+    step. exists a. repeat split; try assumption. lia. 
+    psimpl. now rewrite Cycles.
+
+    (* Addr 0x10 *)
+    destruct PRE as [t0 [T0 [T2 [T3 [T0_A Cycles_t]]]]].
+    step.
+    - (* t0 = 0 -> postcondition *)
+        rewrite N.eqb_eq in BC; subst. unfold_cycle_count_list.
+        unfold_time_of_addr. rewrite T0, T3, Cycles_t. now psimpl.
+    - (* t0 <> 0 -> loop again *)
+        step. step. step. exists (t0 â 1). assert (1 <= t0) by (apply N.eqb_neq in BC; lia). repeat split.
+            rewrite msub_nowrap; psimpl; lia.
+        unfold_cycle_count_list.
+        repeat (let Y := fresh "H" in (remember ((time_of_addr _) _) eqn:Y; unfold_time_of_addr in Y; subst)).
+        rewrite T0, T3, BC, Cycles_t, N.add_sub_assoc, msub_nowrap, N_sub_distr.
+        psimpl. rewrite N.mul_add_distr_r. psimpl.
+        rewrite (N.add_sub_assoc 16).
+
+        all: psimpl; (assumption || lia || apply ML_pos).
+Qed.
